submit

src/inst-semantics.lean
@@ -86,19 +86,20 @@ def refine_bounds [decidable_eq sig] [decidable_eq relation] : list inst → all
 | [] (bounds : all_bounds) := bounds
 | (insthd :: rst) (bounds : all_bounds) := refine_bounds rst (refine_bound insthd bounds)
 
+def new_bounds : all_bounds :=
+(all_bounds.mk (sig_bounds.mk (λx, ∅) (λx, set.univ))
+               (rel_bounds.mk (λx, ∅) (λx, set.univ)))
+
 lemma bounds_conflict_carries_for_sig [decidable_eq sig] [decidable_eq atom] [decidable_eq relation] (s1 : sig) (lower upper : set atom) :
   (lower ⊆ upper) ↔
     ((refine_bounds  [(inst.sig_in_atoms s1 upper), (inst.atoms_in_sig lower s1)]
-                       (all_bounds.mk (sig_bounds.mk (λx, ∅) (λx, set.univ))
-                                      (rel_bounds.mk (λx, ∅) (λx, set.univ)))).sigs.lower s1)
+                      new_bounds).sigs.lower s1)
         ⊆
        ((refine_bounds [(inst.sig_in_atoms s1 upper), (inst.atoms_in_sig lower s1)]
-                       (all_bounds.mk (sig_bounds.mk (λx, ∅) (λx, set.univ))
-                                      (rel_bounds.mk (λx, ∅) (λx, set.univ)))).sigs.upper s1) :=
+                       new_bounds).sigs.upper s1) :=
 begin
   have hlower : lower = (refine_bounds [(inst.sig_in_atoms s1 upper), (inst.atoms_in_sig lower s1)]
-                       (all_bounds.mk (sig_bounds.mk (λx, ∅) (λx, set.univ))
-                                      (rel_bounds.mk (λx, ∅) (λx, set.univ)))).sigs.lower s1 :=
+                       new_bounds).sigs.lower s1 :=
       begin
          calc lower
              = (λ(s : sig), if s = s1 then (lower ∪ ∅) else ∅) s1 :
@@ -111,13 +112,11 @@ begin
                               (rel_bounds.mk (λx, ∅) (λx, set.univ))).sigs.lower s1 :
           by simp
         ... = (refine_bounds [(inst.sig_in_atoms s1 upper), (inst.atoms_in_sig lower s1)]
-                       (all_bounds.mk (sig_bounds.mk (λx, ∅) (λx, set.univ))
-                                      (rel_bounds.mk (λx, ∅) (λx, set.univ)))).sigs.lower s1 :
+                       new_bounds).sigs.lower s1 :
           by refl
       end,
   have hupper : upper = (refine_bounds [(inst.sig_in_atoms s1 upper), (inst.atoms_in_sig lower s1)]
-                       (all_bounds.mk (sig_bounds.mk (λx, ∅) (λx, set.univ))
-                                      (rel_bounds.mk (λx, ∅) (λx, set.univ)))).sigs.upper s1 :=
+                       new_bounds).sigs.upper s1 :=
       begin
          calc upper
              = (λ(s : sig), if s = s1 then (upper ∩ set.univ) else set.univ) s1 :
@@ -130,18 +129,16 @@ begin
                               (rel_bounds.mk (λx, ∅) (λx, set.univ))).sigs.upper s1 :
           by simp
         ... = (refine_bounds [(inst.sig_in_atoms s1 upper), (inst.atoms_in_sig lower s1)]
-                       (all_bounds.mk (sig_bounds.mk (λx, ∅) (λx, set.univ))
-                                      (rel_bounds.mk (λx, ∅) (λx, set.univ)))).sigs.upper s1 :
+                       new_bounds).sigs.upper s1 :
           by refl
       end,
   apply iff.intro,
   { intro hlsubu,
     intro bound,
     intro hboundlower,
-    simp [refine_bounds],
-    simp,
     have hboundeltlower : bound ∈ lower :=
       by cc,
+    rw ←hupper,
     apply hlsubu,
     exact hboundeltlower, },
   { rw ←hupper,
@@ -150,15 +147,79 @@ begin
     exact hlu, },
 end
 
-lemma comm_binary [decidable_eq sig] [decidable_eq atom] [decidable_eq relation]
-  (bounds : all_bounds) (a : inst) (b : inst) :
-  (refine_bounds [a, b] bounds) = (refine_bounds [b, a] bounds) :=
+lemma bounds_conflict_carries_for_rel [decidable_eq sig] [decidable_eq atom] [decidable_eq relation] (r1 : relation) (lower upper : set (list atom)) :
+  (lower ⊆ upper)
+  ↔ ((refine_bounds [(inst.rel_in_atoms r1 upper), (inst.atoms_in_rel lower r1)] new_bounds).rels.lower r1)
+    ⊆ ((refine_bounds [(inst.rel_in_atoms r1 upper), (inst.atoms_in_rel lower r1)] new_bounds).rels.upper r1) :=
 begin
-  
-  sorry
-  
+  have hlower : lower = (refine_bounds [(inst.rel_in_atoms r1 upper), (inst.atoms_in_rel lower r1)]
+                       new_bounds).rels.lower r1 :=
+      begin
+         calc lower
+             = (λ(r : relation), if r = r1 then (lower ∪ ∅) else ∅) r1 :
+          by simp
+        ... = (rel_bounds.mk (λ(r : relation), if r = r1 then (lower ∪ ∅) else ∅)
+                             (λ(r : relation), if r = r1 then (upper ∩ set.univ) else set.univ)).lower r1 :
+          by simp
+         ... = (all_bounds.mk (sig_bounds.mk (λx, ∅) (λx, set.univ))
+                              (rel_bounds.mk (λ(r : relation), if r = r1 then (lower ∪ ∅) else ∅)
+                                             (λ(r : relation), if r = r1 then (upper ∩ set.univ) else set.univ))).rels.lower r1 :
+          by simp
+        ... = (refine_bounds [(inst.rel_in_atoms r1 upper), (inst.atoms_in_rel lower r1)]
+                       new_bounds).rels.lower r1 :
+          by refl
+      end,
+  have hupper : upper = (refine_bounds [(inst.rel_in_atoms r1 upper), (inst.atoms_in_rel lower r1)]
+                         new_bounds).rels.upper r1 :=
+      begin
+         calc upper
+             = (λ(r : relation), if r = r1 then (upper ∩ set.univ) else set.univ) r1 :
+          by simp
+        ... = (rel_bounds.mk (λ(r : relation), if r = r1 then (lower ∪ ∅) else ∅)
+                             (λ(r : relation), if r = r1 then (upper ∩ set.univ) else set.univ)).upper r1 :
+          by simp
+         ... = (all_bounds.mk (sig_bounds.mk (λx, ∅) (λx, set.univ))
+                              (rel_bounds.mk (λ(r : relation), if r = r1 then (lower ∪ ∅) else ∅)
+                                             (λ(r : relation), if r = r1 then (upper ∩ set.univ) else set.univ))).rels.upper r1 :
+          by simp
+        ... = (refine_bounds [(inst.rel_in_atoms r1 upper), (inst.atoms_in_rel lower r1)]
+                       new_bounds).rels.upper r1 :
+          by refl
+      end,
+  apply iff.intro,
+  { intro hlsubu,
+    intro bound,
+    intro hboundlower,
+    have hboundeltlower : bound ∈ lower :=
+      by cc,
+    rw ←hupper,
+    apply hlsubu,
+    exact hboundeltlower, },
+  { rw ←hupper,
+    rw ←hlower,
+    intro hlu,
+    exact hlu, },
 end
 
+/-!
+  We spent about an hour trying to figure this one out
+  Turns out the only good way is to use casework
+  But then you need to do cases on i1 and i2, which gives you at least 16 cases total
+  So we decided it's not worth the time
+-/
+lemma comm_binary [decidable_eq sig] [decidable_eq atom] [decidable_eq relation] (i1 i2 : inst) (bounds : all_bounds) :
+  refine_bounds [i1, i2] bounds = refine_bounds [i2, i1] bounds :=
+sorry
+
+/-!
+  We spent about 3 hours trying to figure this one out
+  We got a proof by hand
+  The proofs required induction with multiple base cases
+  We need the cases where the list has length 1,2, and 3 for this
+  The problem is the case with length 3 we could only do by casework, and we thought it wasn't worth doing the 64 cases that gives us
+  We also could not figure out how to tell lean "we would like to induct, but we want to induct for cases with length >= 3
+  and do the other cases by hand" instead of having it induct on all cases of size >= 1
+-/
 lemma comm [decidable_eq sig] [decidable_eq atom] [decidable_eq relation]
   (bounds : all_bounds) (insthd : inst) (rst : list inst) :
   (refine_bounds (insthd :: rst) bounds) = (refine_bounds (rst.append [insthd]) bounds) :=
@@ -166,5 +227,41 @@ begin
   rw refine_bounds,
   sorry
 end
+
+lemma inst_reverse [decidable_eq sig] [decidable_eq atom] [decidable_eq relation] (i1 i2 i3 : inst) (bound : all_bounds) :
+  refine_bounds [i1, i2, i3] bound = refine_bounds [i3, i2, i1] bound :=
+calc refine_bounds [i1, i2, i3] bound
+    = refine_bounds [i2, i3] (refine_bounds [i1] bound) :
+  by refl
+...  = refine_bounds [i3, i2] (refine_bounds [i1] bound) :
+  by apply comm_binary
+... = refine_bounds [i1, i3, i2] bound :
+  by refl
+... = refine_bounds [i2] (refine_bounds [i1, i3] bound) :
+  by refl
+... = refine_bounds [i2] (refine_bounds [i3, i1] bound) :
+  by simp [comm_binary]
+... = refine_bounds [i3, i1, i2] bound :
+  by refl
+... = refine_bounds [i1, i2] (refine_bounds [i3] bound) :
+  by refl
+... = refine_bounds [i2, i1] (refine_bounds [i3] bound) :
+  by apply comm_binary
+... = refine_bounds [i3, i2, i1] bound:
+  by refl
+
+lemma inst_assoc [decidable_eq sig] [decidable_eq atom] [decidable_eq relation] (i1 i2 i3 : inst) (bounds : all_bounds):
+  refine_bounds [i1] (refine_bounds [i2, i3] bounds) = refine_bounds [i1, i2] (refine_bounds [i3] bounds) :=
+calc refine_bounds [i1] (refine_bounds [i2, i3] bounds)
+    = refine_bounds [i2, i3, i1] bounds:
+  by refl
+...  = refine_bounds [i3, i1] (refine_bounds [i2] bounds) :
+  by refl
+... = refine_bounds [i1, i3] (refine_bounds [i2] bounds) :
+  by apply comm_binary
+... = refine_bounds [i2, i1, i3] bounds :
+  by refl
+... = refine_bounds [i3, i1, i2] bounds :
+  by apply inst_reverse
 
 end LoVe
